new version of steps

theories/example.v
@@ -1,6 +1,11 @@
 Require Import isla.base.
 Require Import isla.opsem.
 
+Ltac solve_trace_step := by econstructor.
+Ltac do_trace_step :=
+  apply: TraceStep'; [solve_trace_step | done |]; simpl.
+
+
 (* trace of add x1, x2, x3:
   (read-reg |R2| nil v3359)
   (define-const v3425 v3359)
@@ -13,7 +18,7 @@ Require Import isla.opsem.
   (define-const v3452 v3437)
   (write-reg |R1| nil v3452)
 *)
-Definition add_x1_x2_x3 : trc :=
+Definition trc_add_x1_x2_x3 : trc :=
   [
   Smt (DeclareConst 3359 (Ty_BitVec 64)) Mk_annot;
   Smt (DeclareConst 3361 (Ty_BitVec 64)) Mk_annot;
@@ -30,23 +35,162 @@ Definition add_x1_x2_x3 : trc :=
 ].
 
 Lemma add_x1_x2_x3_trace bv2 bv3 :
-  add_x1_x2_x3 ~{ trace_module, [
+  trc_add_x1_x2_x3 ~{ trace_module, [
                     Vis (LReadReg "R2" [] (Val_Bits bv2));
                     Vis (LReadReg "R3" [] (Val_Bits bv3));
                     Vis (LWriteReg "R1" [] (Val_Bits (Z_extract 63 0 (bv2 + bv3))))
                 ] }~> [].
 Proof.
-  apply: TraceStepNone. { apply: (DeclareConstS (Val_Bits _)). shelve. } simpl.
-  apply: TraceStepNone. { apply: (DeclareConstS (Val_Bits _)). shelve. } simpl.
-  apply: TraceStepSome. { econstructor. } simpl.
-  apply: TraceStepNone. { by econstructor. } simpl.
-  apply: TraceStepSome. { econstructor. } simpl.
-  apply: TraceStepNone. { by econstructor. } simpl.
-  apply: TraceStepNone. { by econstructor. } simpl.
-  apply: TraceStepNone. { by econstructor. } simpl.
-  apply: TraceStepNone. { by econstructor. } simpl.
-  apply: TraceStepNone. { by econstructor. } simpl.
-  apply: TraceStepNone. { by econstructor. } simpl.
-  apply: TraceStepSome. { econstructor. } simpl.
+  do_trace_step.
+  do_trace_step.
+  do_trace_step.
+  do_trace_step.
+  do_trace_step.
+  do_trace_step.
+  do_trace_step.
+  do_trace_step.
+  do_trace_step.
+  do_trace_step.
+  do_trace_step.
+  do_trace_step.
   by apply: TraceEnd.
+Qed.
+
+(*
+C:
+int test() {
+    return 0;
+}
+compiled via GCC:
+        mov     w0, 0
+        ret
+
+trace of mov w0, 0:
+  (write-reg |R0| nil #x0000000000000000))
+
+trace of ret:
+(trace
+  (declare-const v3428 (_ BitVec 64))
+  (define-const v3429 v3428)
+  (read-reg |R30| nil v3429)
+  (define-const v3435 v3429)
+#  (write-reg |BTypeNext| nil #b00)
+  (define-const v3436 v3435)
+  (branch-address v3436)
+  (define-const v3437 v3435)
+# There are two generated traces, but they seem to do the same
+#  (define-const v3471 (= (bvor #b0 ((_ extract 0 0) (bvlshr v3437 #x0000000000000037))) #b1))
+#  (branch 0 "model/aarch_mem.sail 6170:20 - 6170:81")
+#  (assert v3471)
+  (write-reg |_PC| nil v3437)
+  (write-reg |__PC_changed| nil true))
+*)
+
+Definition trc_mov_w0_0 : trc := [
+   WriteReg "R0" [] (Val_Bits 0x0000000000000000) Mk_annot
+  ].
+
+Definition trc_ret : trc := [
+  Smt (DeclareConst 3428 (Ty_BitVec 64)) Mk_annot;
+  Smt (DefineConst 3429 (Val (Val_Symbolic 3428) Mk_annot)) Mk_annot;
+  ReadReg "R30" nil (Val_Symbolic 3429) Mk_annot;
+  Smt (DefineConst 3435 (Val (Val_Symbolic 3429) Mk_annot)) Mk_annot;
+  (* WriteReg "BTypeNext" nil (Val_Bits 0) Mk_annot; *)
+  Smt (DefineConst 3436 (Val (Val_Symbolic 3435) Mk_annot)) Mk_annot;
+  BranchAddress (Val_Symbolic 3436) Mk_annot;
+  Smt (DefineConst 3437 (Val (Val_Symbolic 3435) Mk_annot)) Mk_annot;
+  WriteReg "_PC" nil (Val_Symbolic 3437) Mk_annot;
+  WriteReg "__PC_changed" nil (Val_Bool true) Mk_annot
+].
+
+(* trace of bl 0x100: (at address 0x0000000010300000)
+(trace
+  (read-reg |_PC| nil #x0000000010300000)
+  (write-reg |R30| nil #x0000000010300004)
+  (read-reg |_PC| nil #x0000000010300000)
+  (branch-address #x0000000010300100)
+  (write-reg |_PC| nil #x0000000010300100)
+  (write-reg |__PC_changed| nil true))
+*)
+Definition trc_bl_0x100 : trc := [
+  ReadReg "_PC" nil (Val_Bits 0x0000000010300000) Mk_annot;
+  WriteReg "R30" nil (Val_Bits 0x0000000010300004) Mk_annot;
+  ReadReg "_PC" nil (Val_Bits 0x0000000010300000) Mk_annot;
+  BranchAddress (Val_Bits 0x0000000010300100) Mk_annot;
+  WriteReg "_PC" nil (Val_Bits 0x0000000010300100) Mk_annot;
+  WriteReg "__PC_changed" nil (Val_Bool true) Mk_annot
+].
+
+(* trace of mov x28, x0:
+trace
+  (declare-const v3368 (_ BitVec 64))
+  (define-const v3369 v3368)
+  (read-reg |R0| nil v3369)
+  (define-const v3450 (bvor #x0000000000000000 v3369))
+  (write-reg |R28| nil v3450))
+
+*)
+Definition trc_mov_x28_x0 : trc := [
+  Smt (DeclareConst 3368 (Ty_BitVec 64)) Mk_annot;
+  Smt (DefineConst 3369 (Val (Val_Symbolic 3368) Mk_annot)) Mk_annot;
+  ReadReg "R0" nil (Val_Symbolic 3369) Mk_annot;
+  Smt (DefineConst 3450 (Manyop (Bvmanyarith Bvor) [Val (Val_Bits 0x0000000000000000) Mk_annot; Val (Val_Symbolic 3369) Mk_annot] Mk_annot)) Mk_annot;
+  WriteReg "R28" nil (Val_Symbolic 3450) Mk_annot
+].
+
+Definition test_state := {|
+  seq_trace  := [];
+  seq_regs   :=
+    <[ "_PC" := Val_Bits (0x0000000010300000 - 0x4) ]> $
+    <[ "__PC_changed" := Val_Bool false ]> $
+     ∅;
+  seq_instrs :=
+    <[0x0000000010300000 := [trc_bl_0x100]]> $
+    <[0x0000000010300004 := [trc_mov_x28_x0]]> $
+    <[0x0000000010300100 := [trc_mov_w0_0]]> $
+    <[0x0000000010300104 := [trc_ret]]> $
+    ∅
+|}.
+
+Arguments insert_regmap _ _ _ /.
+
+Ltac do_seq_step :=
+  apply: TraceStep'; [ econstructor; [solve_trace_step| done] | done |]; simpl.
+
+Ltac do_seq_step_jmp :=
+  apply: TraceStep'; [ econstructor; [solve_trace_step| ];
+                       eexists _, _; repeat (split; first done); vm_compute; split => //; left | done |]; simpl.
+
+Arguments set _ _ _ _ _ _ /.
+
+Lemma test_state_trace :
+  test_state ~{ seq_module test_state, [Vis (SWriteReg "R28" [] (Val_Bits 0)) ] }~> -.
+Proof.
+  eexists _.
+  do_seq_step_jmp.
+  do_seq_step.
+  do_seq_step.
+  do_seq_step.
+  do_seq_step.
+  do_seq_step.
+  do_seq_step.
+  do_seq_step_jmp.
+  do_seq_step.
+  do_seq_step_jmp.
+  do_seq_step.
+  do_seq_step.
+  do_seq_step.
+  do_seq_step.
+  do_seq_step.
+  do_seq_step.
+  do_seq_step.
+  do_seq_step.
+  do_seq_step.
+  do_seq_step_jmp.
+  do_seq_step.
+  do_seq_step.
+  do_seq_step.
+  do_seq_step.
+  do_seq_step.
+  apply: TraceEnd.
 Qed.
